Phi_System/Fiction_Refinement.thy
@@ -1,36 +1,205 @@
 theory Fiction_Refinement
-  imports Spec_Framework
+  imports PhiSem_Formalization_Tools
   abbrevs "<refines>" = "\<r>\<e>\<f>\<i>\<n>\<e>\<s>"
       and "<w.r.t>" = "\<w>.\<r>.\<t>"
 begin
 
-term Id
-term \<open>(O)\<close>
-term \<open>(OO)\<close>
-term Interp
-term \<open>\<I> x\<close>
-thm \<phi>Procedure_def
+
+
+
+
+
+
+
+
+
+
+definition Is_Frame_Proc :: \<open>'ret::VALs proc \<Rightarrow> bool\<close>
+  where \<open>Is_Frame_Proc f \<longleftrightarrow>
+    (\<forall>v s s' r. Success v s' \<in> f s \<and> r ## s \<longrightarrow> Success v (r * s') \<in> f (r * s) \<and> r ## s') \<and>
+    (\<forall>e s s' r. Abnormal e s' \<in> f s \<and> r ## s \<longrightarrow> Abnormal e (r * s') \<in> f (r * s) \<and> r ## s')\<close>
+
+(* definition Is_Frame_Proc :: \<open>'ret::VALs proc \<Rightarrow> bool\<close>
+  where \<open>Is_Frame_Proc f \<longleftrightarrow>
+    (\<forall>v s s' r. Success v s' \<in> f s \<and> r ## s \<longrightarrow> Success v (r * s') \<in> f (r * s) \<and> r ## s') \<and>
+    (\<forall>e s s' r. Abnormal e s' \<in> f s \<and> r ## s \<longrightarrow> Abnormal e (r * s') \<in> f (r * s) \<and> r ## s')\<close> *)
+
+lemma
+  \<open> Is_Frame_Proc F
+\<Longrightarrow> (\<And>v. Is_Frame_Proc (G v))
+\<Longrightarrow> Is_Frame_Proc (F \<bind> G)\<close>
+  unfolding Is_Frame_Proc_def bind_def
+  subgoal premises prems
+    apply (clarsimp; rule; clarsimp)
+    apply (case_tac x; simp add: Bex_def split_comp_Ex)
+    using prems(1) prems(2) apply blast
+    apply (case_tac x; simp add: Bex_def split_comp_Ex)
+    using prems(1) prems(2) apply blast
+    using prems(1) by blast .
+    
+
+definition Valid_Operation :: \<open>'ret::VALs proc \<Rightarrow> bool\<close>
+  where \<open>Valid_Operation f \<longleftrightarrow> (\<forall>v s s'. Success v s' \<in> f s \<and> s \<in> RES.SPACE \<longrightarrow> s' \<in> RES.SPACE)
+                             \<and> (\<forall>e s s'. Abnormal e s' \<in> f s \<and> s \<in> RES.SPACE \<longrightarrow> s' \<in> RES.SPACE)\<close>
+
+lemma
+  \<open> Valid_Operation f
+\<Longrightarrow> (\<And>v. Valid_Operation (g v))
+\<Longrightarrow> Valid_Operation (f \<bind> g)\<close>
+  unfolding Valid_Operation_def bind_def
+  subgoal premises prems
+    apply (clarsimp; rule; clarsimp)
+    apply (case_tac x; simp add: Bex_def split_comp_Ex)
+    using prems(1) prems(2) apply blast
+    apply (case_tac x; simp add: Bex_def split_comp_Ex)
+    using prems(1) prems(2) apply blast
+    using prems(1) by blast .
+  
+
+definition Transition_of :: \<open>'ret::VALs proc \<Rightarrow> 'ret \<phi>arg + ABNM \<Rightarrow> resource rel\<close>
+  where \<open>Transition_of f = (\<lambda>x. case x of Inl v \<Rightarrow> { (s,s'). Success v s' \<in> f s \<and> s \<in> RES.SPACE }
+                                        | Inr e \<Rightarrow> { (s,s'). Abnormal e s' \<in> f s \<and> s \<in> RES.SPACE } )\<close>
+
+declare [[typedef_overloaded]]
+datatype 'ret eval_stat = Normal \<open>'ret \<phi>arg\<close> | Abnm ABNM | Crash
+declare [[typedef_overloaded = false]]
+
+lemma eval_stat_forall:
+  \<open>All P \<longleftrightarrow> (\<forall>ret. P (Normal ret)) \<and> (\<forall>e. P (Abnm e)) \<and> P Crash\<close>
+  by (metis eval_stat.exhaust)
+
+lemma eval_stat_ex:
+  \<open>Ex P \<longleftrightarrow> (\<exists>ret. P (Normal ret)) \<or> (\<exists>e. P (Abnm e)) \<or> P Crash\<close>
+  by (metis eval_stat.exhaust)
+
+
+definition Transition_of' :: \<open>'ret::VALs proc \<Rightarrow> 'ret eval_stat \<Rightarrow> resource rel\<close>
+  where \<open>Transition_of' f = (\<lambda>x. (case x of Normal v \<Rightarrow> { (s,s'). Success v s' \<in> f s \<and> s \<in> RES.SPACE }
+                                          | Abnm e \<Rightarrow> { (s,s'). Abnormal e s' \<in> f s \<and> s \<in> RES.SPACE }
+                                          | Crash \<Rightarrow> { (s,s'). Invalid \<in> f s \<and> s \<in> RES.SPACE }))\<close>
+
+definition Valid_Transition :: \<open>('ret eval_stat \<Rightarrow> 'a rel) \<Rightarrow> bool\<close>
+  where \<open>Valid_Transition tr \<longleftrightarrow> tr Crash = {}\<close>
+
+
+definition Transition_of_Success :: \<open>'ret::VALs proc \<Rightarrow> 'ret \<phi>arg \<Rightarrow> resource rel\<close>
+  where \<open>Transition_of_Success f = (\<lambda>v. { (s,s'). Success v s' \<in> f s })\<close>
+
+
 
 
 definition Raw_Procedure :: "'ret::VALs proc
                         \<Rightarrow> ('ret \<phi>arg \<Rightarrow> resource rel)
                         \<Rightarrow> bool"
     ("\<r>\<a>\<w> \<p>\<r>\<o>\<c> (2_) \<r>\<e>\<f>\<i>\<n>\<e>\<s> _ " [11,11] 10)
-  where "Raw_Procedure f S \<longleftrightarrow> (\<forall>x r. (\<exists>v y. (x,y) \<in> S v) \<longrightarrow> f (r * x) \<subseteq> \<S> (\<lambda>v. { r * y | y. (x,y) \<in> S v }) 0)"
+  where "Raw_Procedure f S \<longleftrightarrow> (\<forall>x r. f (r * x) \<subseteq> \<S> (\<lambda>v. { r * y | y. (x,y) \<in> S v }) 0)"
+
+definition Fictional_Refine :: "'ret::VALs proc
+                        \<Rightarrow> ('ret \<phi>arg \<Rightarrow> fiction rel)
+                        \<Rightarrow> bool"
+  where \<open>Fictional_Refine f S \<longleftrightarrow> (\<forall>x r. f (r * x) \<subseteq> \<S> (\<lambda>v. { r * y | y. (x,y) \<in> S v }) 0)\<close>
 
 term Domain
 
-definition Sep_Forward_Simulation :: \<open>'c rel \<Rightarrow> 'a rel \<Rightarrow> ('a::sep_magma_1,'c::sep_magma_1) interp \<Rightarrow> bool\<close>
+definition Fictional_Forward_Simulation :: \<open>'c rel \<Rightarrow> 'a rel \<Rightarrow> ('a::sep_magma_1,'c::sep_magma_1) interp \<Rightarrow> bool\<close>
       ("_ \<r>\<e>\<f>\<i>\<n>\<e>\<s> _ \<w>.\<r>.\<t> _ " [11,11,11] 10)
-  where \<open>(F \<r>\<e>\<f>\<i>\<n>\<e>\<s> G \<w>.\<r>.\<t> T) \<longleftrightarrow> (\<forall>x r. F `` \<I> T (r * x) \<subseteq> {y'. \<exists>y. y' \<in> \<I> T (r * y) \<and> (x,y) \<in> G})\<close>
+  where \<open>(F \<r>\<e>\<f>\<i>\<n>\<e>\<s> G \<w>.\<r>.\<t> T) \<longleftrightarrow> (\<forall>x r R. F `` (R * \<I> T (r * x) \<s>\<u>\<b>\<j> r ## x) \<subseteq> { y'. \<exists>y. y' \<in> R * \<I> T (r * y) \<and> r ## y \<and> (x,y) \<in> G})\<close>
+
+lemma sep_refinement_stepwise:
+  \<open> S1 \<r>\<e>\<f>\<i>\<n>\<e>\<s> S2 \<w>.\<r>.\<t> I1
+\<Longrightarrow> S2 \<r>\<e>\<f>\<i>\<n>\<e>\<s> S3 \<w>.\<r>.\<t> I2
+\<Longrightarrow> S1 \<r>\<e>\<f>\<i>\<n>\<e>\<s> S3 \<w>.\<r>.\<t> (I1 o\<^sub>\<I> I2)\<close>
+  for S1 :: \<open>'a::sep_monoid rel\<close>
+  and S2 :: \<open>'b::sep_monoid rel\<close>
+  and S3 :: \<open>'c::sep_monoid rel\<close>
+  unfolding Fictional_Forward_Simulation_def interp_comp_\<I>
+  apply (auto simp add: subset_iff Image_def Bex_def \<phi>expns split_option_all)
+  by (smt mult_1_class.mult_1_left sep_magma_1_right set_in_1)
+
+lemma sep_refinement_horizontal_stepwise:
+  \<open> A1 \<r>\<e>\<f>\<i>\<n>\<e>\<s> B1 \<w>.\<r>.\<t> I
+\<Longrightarrow> A2 \<r>\<e>\<f>\<i>\<n>\<e>\<s> B2 \<w>.\<r>.\<t> I
+\<Longrightarrow> A1 O A2 \<r>\<e>\<f>\<i>\<n>\<e>\<s> B1 O B2 \<w>.\<r>.\<t> I\<close>
+  unfolding Fictional_Forward_Simulation_def
+  apply (clarsimp simp add: \<phi>expns subset_iff Image_def Bex_def)
+  by (smt (z3) relcomp.relcompI)
+
+
+
+context resource begin
+
+
+
+end
+
+
+context basic_fiction begin
 
 lemma
-  \<open>A1 \<i>\<m>\<p>\<l>\<i>\<e>\<s> B1 \<w>.\<r>.\<t> T\<close>
+  \<open> Valid_Operation f
+\<Longrightarrow> (\<And>v. Transition_of' f v \<r>\<e>\<f>\<i>\<n>\<e>\<s> S2 v \<w>.\<r>.\<t> R.basic_fiction o\<^sub>\<I> I)
+\<Longrightarrow> Valid_Transition S2
+\<Longrightarrow> \<p>\<r>\<o>\<c> f \<lbrace> x \<Ztypecolon> \<phi> Identity \<longmapsto> \<lambda>v. y \<Ztypecolon> \<phi> Identity \<s>\<u>\<b>\<j> y. (x,y) \<in> S2 (Normal v) \<rbrace> \<t>\<h>\<r>\<o>\<w>\<s> (\<lambda>e. y \<Ztypecolon> \<phi> Identity \<s>\<u>\<b>\<j> y. (x,y) \<in> S2 (Abnm e))\<close>
+  unfolding \<phi>Procedure_alt Fictional_Forward_Simulation_def atomize_all Valid_Transition_def
+  apply (auto simp add: Image_iff subset_iff Bex_def R.basic_fiction_\<I> \<phi>expns Transition_of'_def
+          LooseStateSpec_def split_sum_all INTERP_RES_def interp_split' R.\<r>_valid_split' interp_comp_\<I>
+          R.inject_wand_homo inject_wand_homo prj.homo_mult eval_stat_forall split: eval_stat.split)
+  subgoal premises prems for r u y v y' rr
+    thm prems
+    thm prems(3)[THEN spec[where x=v], THEN spec[where x=x], THEN spec[where x=\<open>get r\<close>], THEN spec[where x=\<open>{u}\<close>], THEN spec[where x=\<open>y'\<close>]]
+  proof -
+    have [simp]: \<open>R.clean y' \<in> R.SPACE\<close>
+      by (metis R.\<r>_valid_split R.inj.homo_mult Valid_Operation_def prems(1) prems(13) prems(14) prems(15) prems(8) prems(9) times_fupdt_1_apply_sep times_fupdt_1_fupdt_1_sep)
+    have t2: \<open>(\<exists>xa. (\<exists>ua v. xa = ua * v \<and> ua \<in> {u} \<and> (\<exists>xa. xa \<in> \<I> I (get r * x) \<and> v = R.mk xa) \<and> ua ## v) \<and>
+      get r ## x \<and> Success v y' \<in> f xa \<and> R.clean xa \<in> R.SPACE \<and> (\<exists>m. xa R.name = R.inject m \<and> m \<in>\<^sub>S R.domain))\<close>
+      apply (rule exI[where x=\<open>(u * R.mk y)\<close>], simp add: prems R.inj.homo_mult[symmetric] )
+      using prems(11) prems(12) by blast
+    note prems(3)[THEN spec[where x=v], THEN spec[where x=x], THEN spec[where x=\<open>get r\<close>], THEN spec[where x=\<open>{u}\<close>], THEN spec[where x=\<open>y'\<close>],
+            THEN mp, OF this]
+    then show ?thesis
+    apply clarsimp
+    subgoal for yy ya
+      apply (rule exI[where x=yy], clarsimp simp add: inj.homo_mult[symmetric] prems prj.homo_mult, rule)
+      apply (metis R.\<r>_valid_split Valid_Operation_def prems(1) prems(14) t2 times_fupdt_1_apply_sep)
+      using prems(10) by blast .
+qed
+  subgoal premises prems for r u y v y' rr
+  proof -
+    thm prems(4)[THEN spec[where x=v], THEN spec[where x=x], THEN spec[where x=\<open>get r\<close>], THEN spec[where x=\<open>{u}\<close>], THEN spec[where x=\<open>y'\<close>]]
+    have [simp]: \<open>R.clean y' \<in> R.SPACE\<close>
+      by (metis R.\<r>_valid_split R.inj.homo_mult Valid_Operation_def prems(1) prems(13) prems(14) prems(15) prems(8) prems(9) times_fupdt_1_apply_sep times_fupdt_1_fupdt_1_sep)
+    have t2: \<open>(\<exists>xa. (\<exists>ua v. xa = ua * v \<and> ua \<in> {u} \<and> (\<exists>xa. xa \<in> \<I> I (get r * x) \<and> v = R.mk xa) \<and> ua ## v) \<and>
+      get r ## x \<and> Abnormal v y' \<in> f xa \<and> R.clean xa \<in> R.SPACE \<and> (\<exists>m. xa R.name = R.inject m \<and> m \<in>\<^sub>S R.domain))\<close>
+      using R.inj.homo_mult prems(11) prems(12) prems(13) prems(14) prems(15) prems(6) prems(7) prems(8) prems(9) by force
+    note prems(4)[THEN spec[where x=v], THEN spec[where x=x], THEN spec[where x=\<open>get r\<close>], THEN spec[where x=\<open>{u}\<close>], THEN spec[where x=\<open>y'\<close>],
+            THEN mp, OF this]
+    then show ?thesis
+      apply clarsimp
+      subgoal for yy ya
+        apply (rule exI[where x=yy], clarsimp simp add: inj.homo_mult[symmetric] prems prj.homo_mult, rule)
+        apply (metis R.\<r>_valid_split Valid_Operation_def prems(1) prems(14) t2 times_fupdt_1_apply_sep)
+        using prems(10) by blast .
+  qed
+  by (metis (mono_tags, lifting) R.inj.homo_mult sep_disj_get_name times_fupdt_1_apply_sep times_fupdt_1_fupdt_1_sep)
+
+
 
 lemma
   \<open> \<r>\<a>\<w> \<p>\<r>\<o>\<c> f \<r>\<e>\<f>\<i>\<n>\<e>\<s> S1
-\<Longrightarrow> (\<And>v. S1 v \<r>\<e>\<f>\<i>\<n>\<e>\<s> S2 \<w>.\<r>.\<t> T)
-\<close>
+\<Longrightarrow> (\<And>v. S1 v \<r>\<e>\<f>\<i>\<n>\<e>\<s> S2 \<w>.\<r>.\<t> (R.basic_fiction I))
+\<Longrightarrow> \<p>\<r>\<e>\<m>\<i>\<s>\<e> x \<in> Domain S2
+\<Longrightarrow> \<p>\<r>\<o>\<c> f \<lbrace> x \<Ztypecolon> \<phi> Identity \<longmapsto> y \<Ztypecolon> \<phi> Identity \<s>\<u>\<b>\<j> y. (x,y) \<in> S2 \<rbrace>\<close>
+  unfolding \<phi>Procedure_Hybrid_DL Raw_Procedure_def Premise_def Sep_Forward_Simulation_def
+  apply (clarsimp simp add: Image_def Bex_def subset_iff
+          zero_set_def zero_fun_def R.basic_fiction_\<I> INTERP_RES_def
+          interp_split' \<r>_valid_split' R.inject_wand_homo inject_wand_homo
+          sep_disj_get_name_eq[symmetric])
+  thm sep_disj_get_name_eq[symmetric]
+  thm inject_wand_homo[OF _ sep_disj_mk_name]
+  thm
+  thm interp_spl
+
+end
 
 
 lemma
