Phi_System/PhiSem_Formalization_Tools.thy
@@ -252,19 +252,20 @@ lemma get_res_Valid:
 \<Longrightarrow> get res \<in>\<^sub>S domain\<close>
   unfolding \<phi>Res_Spec_def \<phi>Res_Sat_def by (clarsimp simp add: \<r>_valid_split')
 
+definition \<open>basic_fiction = Interp (\<lambda>x. { 1(Res #= x)})\<close>
 
-definition \<open>basic_fiction I = Interp (\<lambda>x. { 1(Res #= y) |y. y \<in> \<I> I x })\<close>
 lemma basic_fiction_\<I>:
-  "\<I> (basic_fiction I) = (\<lambda>x. { 1(Res #= y) |y. y \<in> \<I> I x})"
+  "\<I> basic_fiction = (\<lambda>x. { 1(Res #= x)})"
   unfolding basic_fiction_def
   by (rule Interp_inverse) (clarsimp simp add: Interpretation_def one_set_def)
 
+
 lemma \<F>_itself_expn[\<phi>expns]:
   \<open>R2 ## x
-\<Longrightarrow> \<phi>Res_Spec (\<I> (basic_fiction \<F>_it) (R2 * x))
-  = \<phi>Res_Spec (\<I> (basic_fiction \<F>_it) R2 * {mk x})\<close>
+\<Longrightarrow> \<phi>Res_Spec (\<I> (basic_fiction \<circ>\<^sub>\<I> \<F>_it) (R2 * x))
+  = \<phi>Res_Spec (\<I> (basic_fiction \<circ>\<^sub>\<I> \<F>_it) R2 * {mk x})\<close>
   unfolding \<phi>Res_Spec_def set_eq_iff
-  apply (clarsimp simp add: \<phi>expns basic_fiction_\<I> prj.homo_mult)
+  apply (clarsimp simp add: \<phi>expns basic_fiction_\<I> prj.homo_mult interp_comp_\<I>)
   apply (rule; clarify)
    apply (simp add: mk_homo_mult sep_mult_assoc')
   using SPACE_mult_homo inj.homo_mult by force
@@ -284,7 +285,7 @@ subsubsection \<open>Basic Fiction\<close>
 
 locale basic_fiction =
    R: resource Res
-+  fiction_kind FIC.DOMAIN INTERPRET Fic \<open>R.basic_fiction I\<close>
++  fiction_kind FIC.DOMAIN INTERPRET Fic \<open>R.basic_fiction \<circ>\<^sub>\<I> I\<close>
 for Res :: "'T::sep_algebra resource_entry"
 and I :: "('U::sep_algebra, 'T) interp"
 and Fic :: "'U fiction_entry"
@@ -462,7 +463,7 @@ locale permission_fiction =
    R: resource Res
 +  share: perm_ins_homo_L \<psi>
 +  fiction_kind FIC.DOMAIN INTERPRET Fic
-      \<open>R.basic_fiction (\<F>_functional \<psi>)\<close>
+      \<open>R.basic_fiction \<circ>\<^sub>\<I> (\<F>_functional \<psi>)\<close>
 for Res :: "'T::sep_algebra resource_entry"
 and \<psi> :: \<open>'T \<Rightarrow> 'U::{share_sep_disj,share_module_sep,sep_algebra}\<close>
 and Fic :: "'U fiction_entry"
@@ -475,7 +476,7 @@ lemma sep_disj_fiction:
 \<Longrightarrow> \<s>\<t>\<a>\<t>\<e> s \<i>\<s> \<I> INTERP r * { R.mk x }
 \<Longrightarrow> r ## mk (\<psi> x)\<close>
   unfolding \<phi>Res_Sat_def \<phi>Res_Spec_def set_eq_iff
-  apply (clarsimp simp add: R.basic_fiction_\<I> \<phi>expns
+  apply (clarsimp simp add: R.basic_fiction_\<I> interp_comp_\<I> \<phi>expns
             \<phi>Res_Spec_def R.\<r>_valid_split'
             R.inject_wand_homo interp_split'
             sep_disj_get_name_eq[symmetric]
@@ -488,7 +489,7 @@ lemma expand_subj:
   = \<phi>Res_Spec (\<I> INTERP r * { R.mk x })\<close>
   unfolding \<phi>Res_Spec_def set_eq_iff
   apply (clarify, rule)
-  apply (clarsimp simp add: R.basic_fiction_\<I> \<phi>expns
+  apply (clarsimp simp add: R.basic_fiction_\<I> interp_comp_\<I> \<phi>expns
             share.homo_sep_wand \<phi>Res_Spec_def R.\<r>_valid_split'
             R.inject_wand_homo interp_split' prj.homo_mult)
   thm interp_split'
@@ -498,7 +499,7 @@ lemma expand_subj:
     by (metis R.mk_homo_mult R.sep_disj_mk sep_disj_multD1 sep_disj_multI1)
 
   apply (clarsimp simp add: R.basic_fiction_\<I> \<phi>expns \<phi>Res_Spec_def R.\<r>_valid_split'
-        R.inject_wand_homo interp_split' sep_mult_assoc prj.homo_mult)
+        R.inject_wand_homo interp_split' sep_mult_assoc prj.homo_mult interp_comp_\<I>)
   subgoal premises prems for res_r a y proof -
     have t1[simp]: \<open>y ## x\<close>
       using prems(5) prems(7) sep_disj_multD2 by force
@@ -536,7 +537,7 @@ lemma partial_implies_raw:
 \<Longrightarrow> \<s>\<t>\<a>\<t>\<e> res \<i>\<s> \<I> INTERP (r * mk (share n (\<psi> x)))
 \<Longrightarrow> x \<preceq>\<^sub>S\<^sub>L R.get res\<close>
   unfolding \<phi>Res_Spec_def \<phi>Res_Sat_def
-  apply (clarsimp simp add: R.basic_fiction_\<I> \<phi>expns
+  apply (clarsimp simp add: R.basic_fiction_\<I> interp_comp_\<I> \<phi>expns
             \<phi>Res_Spec_def R.\<r>_valid_split' R.inject_wand_homo
             R.prj.homo_mult interp_split' prj.homo_mult)
   apply (cases \<open>n \<le> 1\<close>)
@@ -572,7 +573,7 @@ subsubsection \<open>Identity Fiction\<close>
 
 locale identity_fiction =
    R: resource Res
-+  fiction_kind FIC.DOMAIN INTERPRET Fic \<open>R.basic_fiction \<F>_it\<close>
++  fiction_kind FIC.DOMAIN INTERPRET Fic \<open>R.basic_fiction o\<^sub>\<I> \<F>_it\<close>
 for Res :: "'T::sep_algebra resource_entry"
 and Fic :: "'T fiction_entry"
 begin
@@ -584,7 +585,7 @@ lemma sep_disj_fiction:
 \<Longrightarrow> \<s>\<t>\<a>\<t>\<e> s \<i>\<s> \<I> INTERP r * { R.mk x }
 \<Longrightarrow> r ## mk x\<close>
   unfolding \<phi>Res_Sat_def \<phi>Res_Spec_def set_eq_iff
-  apply (clarsimp simp add: R.basic_fiction_\<I> \<phi>expns
+  apply (clarsimp simp add: R.basic_fiction_\<I> interp_comp_\<I> \<phi>expns
             \<phi>Res_Spec_def R.\<r>_valid_split'
             R.inject_wand_homo interp_split'
             sep_disj_get_name_eq[symmetric]
@@ -595,9 +596,9 @@ lemma expand_subj:
   \<open> r \<in> FIC.SPACE
 \<Longrightarrow> (\<phi>Res_Spec (\<I> INTERP (r * mk x) \<s>\<u>\<b>\<j> r ## mk x)) = \<phi>Res_Spec (\<I> INTERP r * {R.mk x}) \<close>
   unfolding \<phi>Res_Spec_def set_eq_iff
-  apply (clarify; rule; clarsimp simp add: \<phi>expns R.basic_fiction_\<I> interp_split' prj.homo_mult)
+  apply (clarify; rule; clarsimp simp add: \<phi>expns R.basic_fiction_\<I> interp_split' prj.homo_mult interp_comp_\<I>)
   apply (simp add: R.mk_homo_mult)
-  using R.sep_disj_mk sep_disj_get_name_eq sep_disj_multD1 sep_disj_multI1 sep_mult_assoc' apply blast
+  apply (metis (no_types, lifting) R.sep_disj_mk sep_disj_get_name sep_disj_multD1 sep_disj_multI1 sep_mult_assoc')
   apply (simp add: R.mk_homo_mult[symmetric] sep_mult_assoc)
   by (metis R.mk_homo_mult R.sep_disj_mk sep_disj_get_name_eq sep_disj_multD2 sep_disj_multI2)
 
@@ -625,7 +626,7 @@ for Res :: "'T nosep option resource_entry"
 begin
 
 definition fiction_agree
-  where \<open>fiction_agree = basic_fiction (\<F>_optionwise \<F>_agree)\<close>
+  where \<open>fiction_agree = basic_fiction o\<^sub>\<I> \<F>_optionwise \<F>_agree\<close>
 
 end
 
@@ -654,7 +655,7 @@ lemma partial_implies:
 \<Longrightarrow> R.get res = Some (nosep x)\<close>
   unfolding \<phi>Res_Spec_def \<phi>Res_Sat_def
   apply (clarsimp simp add: interp_split'
-     R.fiction_agree_def R.basic_fiction_\<I> \<phi>expns R.\<r>_valid_split'
+     R.fiction_agree_def R.basic_fiction_\<I> interp_comp_\<I> \<phi>expns R.\<r>_valid_split'
      R.inject_wand_homo R.prj.homo_mult \<F>_optionwise_\<I> image_iff Bex_def
      \<F>_agree_def prj.homo_mult)
   apply (cases \<open>get r\<close>; simp)
@@ -788,7 +789,7 @@ lemma "__dispose_rule__":
 
 abbreviation perm_ins_homo :: \<open>('key \<Rightarrow> 'val option) \<Rightarrow> ('key \<Rightarrow> 'val share option)\<close>
   where \<open>perm_ins_homo \<equiv> (o) to_share\<close>
-abbreviation \<open>share_fiction \<equiv> basic_fiction (\<F>_functional perm_ins_homo)\<close>
+abbreviation \<open>share_fiction \<equiv> basic_fiction o\<^sub>\<I> \<F>_functional perm_ins_homo\<close>
 
 (* lemma share_fiction_expn_full:
   \<open>\<phi>Res_Spec (R * \<I> share_fiction (R2 * Fine (1(k \<mapsto> 1 \<Znrres> v))))
@@ -848,7 +849,7 @@ subsubsection \<open>Identity Fiction\<close>
 
 locale identity_fiction_for_partial_mapping_resource =
    R: partial_map_resource Res
-+  fiction_kind FIC.DOMAIN INTERPRET Fic \<open>R.basic_fiction \<F>_it\<close>
++  fiction_kind FIC.DOMAIN INTERPRET Fic \<open>R.basic_fiction o\<^sub>\<I> \<F>_it\<close>
 for Res :: "('key \<Rightarrow> 'val::nonsepable_semigroup option) resource_entry"
 and Fic :: "('key \<Rightarrow> 'val option) fiction_entry"
 begin
@@ -1019,7 +1020,7 @@ lemma "__dispose_rule__":
 
 abbreviation perm_ins_homo :: \<open>('key \<Rightarrow> 'key2 \<Rightarrow> 'val option) \<Rightarrow> ('key \<Rightarrow> 'key2 \<Rightarrow> 'val share option)\<close>
   where \<open>perm_ins_homo \<equiv> (o) ((o) to_share)\<close>
-abbreviation \<open>share_fiction \<equiv> basic_fiction (\<F>_functional perm_ins_homo)\<close>
+abbreviation \<open>share_fiction \<equiv> basic_fiction o\<^sub>\<I> \<F>_functional perm_ins_homo\<close>
 
 (*depreciated!*)
 (*lemma share_fiction_expn_full':
@@ -1183,10 +1184,10 @@ lemma [\<phi>reason 1200 for \<open>?R \<heavy_comma> ?x \<Ztypecolon> Val ?raw 
   by (clarsimp simp add: \<phi>expns)
 
 
-subsection \<open>Abnormality\<close>
+subsection \<open>Abnormal\<close>
 
 definition throw :: \<open>ABNM \<Rightarrow> 'ret::VALs proc\<close>
-  where \<open>throw raw = det_lift (Abnormality raw)\<close>
+  where \<open>throw raw = det_lift (Abnormal raw)\<close>
 
 lemma throw_reduce_tail[procedure_simps,simp]:
   \<open>(throw any \<ggreater> f) = throw any\<close>
@@ -1208,7 +1209,7 @@ lemma throw_\<phi>app:
 
 definition op_try :: "'ret proc \<Rightarrow> (ABNM \<Rightarrow> 'ret proc) \<Rightarrow> 'ret::VALs proc"
   where \<open>op_try f g s = \<Union>((\<lambda>y. case y of Success x s' \<Rightarrow> {Success x s'}
-                                       | Abnormality v s' \<Rightarrow> g v s'
+                                       | Abnormal v s' \<Rightarrow> g v s'
                                        | AssumptionBroken \<Rightarrow> {AssumptionBroken}
                                        | NonTerm \<Rightarrow> {NonTerm}
                                        | Invalid \<Rightarrow> {Invalid}) ` f s)\<close>
@@ -1224,7 +1225,7 @@ lemma "__op_try__"[intro!]:
       using prems(1)[THEN spec[where x=comp], THEN spec[where x=R]]
       by (metis (no_types, lifting) INTERP_SPEC LooseStateSpec_expn(1) prems(3) prems(6) prems(7) prems(8) prems(9) set_mult_expn)
     subgoal premises prems for a b c d u v2 proof -
-      have \<open>Abnormality a b \<in> \<S> (\<lambda>v. INTERP_SPEC (R \<heavy_comma> Y1 v)) (\<lambda>v. INTERP_SPEC (R \<heavy_comma> E v))\<close>
+      have \<open>Abnormal a b \<in> \<S> (\<lambda>v. INTERP_SPEC (R \<heavy_comma> Y1 v)) (\<lambda>v. INTERP_SPEC (R \<heavy_comma> E v))\<close>
         using prems(1)[THEN spec[where x=comp], THEN spec[where x=R]]
         using prems(10) prems(3) prems(7) prems(8) prems(9) by blast
       note this[simplified]
@@ -1236,11 +1237,11 @@ lemma "__op_try__"[intro!]:
         by (metis INTERP_SPEC prems(11) set_mult_expn)
     qed
     subgoal premises prems for a b c d u v proof -
-      have \<open>Abnormality a b \<in> \<S> (\<lambda>v. INTERP_SPEC (R \<heavy_comma> Y1 v)) (\<lambda>v. INTERP_SPEC (R \<heavy_comma> E v))\<close>
+      have \<open>Abnormal a b \<in> \<S> (\<lambda>v. INTERP_SPEC (R \<heavy_comma> Y1 v)) (\<lambda>v. INTERP_SPEC (R \<heavy_comma> E v))\<close>
         using prems(1)[THEN spec[where x=comp], THEN spec[where x=R]]
         using prems(10) prems(3) prems(7) prems(8) prems(9) by blast
       note this[simplified]
-      then have \<open>Abnormality c d \<in> \<S> (\<lambda>v. INTERP_SPEC (R \<heavy_comma> Y2 v)) (\<lambda>v. INTERP_SPEC (R \<heavy_comma> E2 v))\<close>
+      then have \<open>Abnormal c d \<in> \<S> (\<lambda>v. INTERP_SPEC (R \<heavy_comma> Y2 v)) (\<lambda>v. INTERP_SPEC (R \<heavy_comma> E2 v))\<close>
         using prems(2)[THEN spec[where x=b], THEN spec[where x=R]]
         by (meson INTERP_SPEC prems(4) set_mult_expn)
       note this[simplified]
